\documentclass[a4paper]{article}

\usepackage{amsmath}

\begin{document}

\[
r'_i \equiv r_i - b_i
\]

\[
\left[
  \begin{array}{cccc}
    1 & 1 & 0 & 0\\
    0 & 0 & 1 & 1\\
    1 & 0 & 1 & 0\\
    0 & 1 & 0 & 1
  \end{array}
  \right]
\left[\begin{array}{c} n_{1\chi} \\ n_{1\phi} \\ n_{2\chi} \\ n_{2\phi}  \end{array}\right]
= 
\left[\begin{array}{c} r'_1 - n_{12}\\ r'_2 - n_{12}\\ r'_\chi - n_{\chi\phi}\\ r'_\phi - n_{\chi\phi} \end{array}\right]
\equiv 
\left[\begin{array}{c} r''_1\\ r''_2\\ r''_\chi\\ r''_\phi \end{array}\right]
\]

\[
D =
\left|
\begin{array}{cccc}
  1 & 1 & 0 & 0\\
  0 & 0 & 1 & 1\\
  1 & 0 & 1 & 0\\
  0 & 1 & 0 & 1
\end{array}
\right|
=
\left|
\begin{array}{ccc}
  0 & 1 & 1\\
  0 & 1 & 0\\
  1 & 0 & 1
\end{array}
\right|
+
\left|
\begin{array}{ccc}
  1 & 0 & 0\\
  0 & 1 & 1\\
  1 & 0 & 1
\end{array}
\right|
=
\left|
\begin{array}{cc}
  1 & 1\\
  1 & 0
\end{array}
\right|
+
\left|
\begin{array}{cc}
1 & 1\\
0 & 1
\end{array}
\right|
= -1 + 1 = 0
\]

\hline

\begin{eqnarray*}
  r'_1 & = & n_{12} + n_{1\chi} + n_{1\phi}\\
  r'_2 & = & n_{12} + n_{2\chi} + n_{2\phi}\\
  r'_\chi & = & n_{1\chi} + n_{2\chi} + n_{\chi\phi}\\
  r'_\phi & = & n_{1\phi} + n_{2\phi} + n_{\chi\phi}
\end{eqnarray*}

\[
n_{12} \le r'_1, r'_2 \qquad n_{\chi\phi} \le r'_\chi, r'_\phi
\]

\[
n_{1\chi} = r'_1 - n_{12} - n_{1\phi} \qquad \boxed{ n_{2\chi} = r'_2 - n_{12} - n_{2\phi} }
\]

\[
\boxed{ n_{1\phi} = r'_\phi - n_{\chi\phi} - n_{2\phi} }
\]

\[
\boxed{ n_{1\chi} = r'_1 - r'_\phi - n_{12} + n_{\chi\phi} + n_{2\phi} }
\]

\[

\]

\hline


\[
\Rightarrow r'_1 + r'_2 - r'_\chi - r'_\phi = 2(n_{12} - n_{\chi\phi})
\]
\[
\Rightarrow \boxed{ n_{12} = \frac{1}{2}\left[r'_1 + r'_2 - r'_\chi - r'_\phi\right] + n_{\chi\phi} }
\]

\[
\Rightarrow \boxed{ n_{1\chi} = \frac{1}{2}\left[r'_\chi + r'_\phi + r'_1 - r'_2\right] - n_{\chi\phi} - n_{1\phi} }
\]
\[
\Rightarrow n_{2\chi} = \frac{1}{2}\left[r'_\chi + r'_\phi + r'_2 - r'_1\right] - n_{\chi\phi} - n_{2\phi}
\]
\[
\Rightarrow \boxed{ n_{2\chi} = \frac{1}{2}\left[r'_\chi - r'_\phi + r'_2 - r'_1\right] + n_{1\phi} }
\]
\[
\boxed{ n_{2\phi} = r'_\phi - n_{\chi\phi} - n_{1\phi} }
\]

\begin{eqnarray*}
  \Rightarrow n_{1\chi} & = & \frac{1}{2}\left[r'_\chi - r'_\phi + r'_1 - r'_2\right] + n_{2\phi} = r'_\chi - n_{2\chi} - n_{\chi\phi}\\
  \Rightarrow n_{2\chi} & = & \frac{1}{2}\left[r'_\chi - r'_\phi + r'_2 - r'_1\right] + n_{1\phi} = r'_\chi - n_{1\chi} - n_{\chi\phi}
\end{eqnarray*}

\[
\boxed{ n_{1\chi} = \frac{1}{2}\left[r'_\chi + r'_\phi + r'_1 - r'_2\right] - n_{1\phi} - n_{\chi\phi} }
\]
\[
n_{1\phi} = \frac{1}{2}\left[ r'_\chi + r'_\phi + r'_1 - r'_2 \right] - n_{\chi\phi} - n_{1\chi}
\]


\end{document}
